src/Std/Tactic/BVDecide/Bitblast/BVExpr/Circuit/Impl.lean
@@ -4,7 +4,25 @@ Released under Apache 2.0 license as described in the file LICENSE.
 Authors: Henrik Böving
 -/
 prelude
-import Std.Tactic.BVDecide.Bitblast.BVExpr.Circuit.Impl.Pred
+import Std.Tactic.BVDecide.Bitblast.BVExpr.Circuit.Impl.Var
+import Std.Tactic.BVDecide.Bitblast.BVExpr.Circuit.Impl.Const
+import Std.Tactic.BVDecide.Bitblast.BVExpr.Circuit.Impl.Operations.Not
+import Std.Tactic.BVDecide.Bitblast.BVExpr.Circuit.Impl.Operations.ShiftLeft
+import Std.Tactic.BVDecide.Bitblast.BVExpr.Circuit.Impl.Operations.ShiftRight
+import Std.Tactic.BVDecide.Bitblast.BVExpr.Circuit.Impl.Operations.Add
+import Std.Tactic.BVDecide.Bitblast.BVExpr.Circuit.Impl.Operations.ZeroExtend
+import Std.Tactic.BVDecide.Bitblast.BVExpr.Circuit.Impl.Operations.Append
+import Std.Tactic.BVDecide.Bitblast.BVExpr.Circuit.Impl.Operations.Replicate
+import Std.Tactic.BVDecide.Bitblast.BVExpr.Circuit.Impl.Operations.Extract
+import Std.Tactic.BVDecide.Bitblast.BVExpr.Circuit.Impl.Operations.RotateLeft
+import Std.Tactic.BVDecide.Bitblast.BVExpr.Circuit.Impl.Operations.RotateRight
+import Std.Tactic.BVDecide.Bitblast.BVExpr.Circuit.Impl.Operations.SignExtend
+import Std.Tactic.BVDecide.Bitblast.BVExpr.Circuit.Impl.Operations.Mul
+import Std.Tactic.BVDecide.Bitblast.BVExpr.Circuit.Impl.Operations.Udiv
+import Std.Tactic.BVDecide.Bitblast.BVExpr.Circuit.Impl.Operations.Umod
+import Std.Tactic.BVDecide.Bitblast.BVExpr.Circuit.Impl.Operations.Eq
+import Std.Tactic.BVDecide.Bitblast.BVExpr.Circuit.Impl.Operations.Ult
+import Std.Tactic.BVDecide.Bitblast.BVExpr.Circuit.Impl.Operations.GetLsbD
 
 -- TODO
 
@@ -18,45 +36,435 @@ This module contains the logic to turn a `BoolExpr Nat` into an `AIG` with maxim
 through the use of a cache that re-uses sub-circuits if possible.
 -/
 
+/-!
+This module contains the implementation of a bitblaster for `BitVec` expressions (`BVExpr`).
+That is, expressions that evaluate to `BitVec` again. Its used as a building block in bitblasting
+general `BitVec` problems with boolean substructure.
+-/
+
+
 
 namespace Std.Tactic.BVDecide
 
-open Std.Sat Std.Sat.AIG
+open Std.Sat
+
+mutual
+
+def BVExpr.bitblast.go {w : Nat} (aig : AIG BVBit) (expr : BVExpr w) :
+    AIG.ExtendingRefVecEntry aig w :=
+  match expr with
+  | .var a =>
+    let res := BVExpr.bitblast.blastVar aig ⟨a⟩
+    ⟨res, AIG.LawfulVecOperator.le_size (f := BVExpr.bitblast.blastVar) ..⟩
+  | .const val =>
+    let res := BVExpr.bitblast.blastConst aig val
+    ⟨res, AIG.LawfulVecOperator.le_size (f := BVExpr.bitblast.blastConst) ..⟩
+  | .ofBool logical =>
+    let ⟨res, _⟩ := BVLogicalExpr.bitblast.go aig logical
+    let aig := res.aig
+    let ref := res.ref
+    let vec := AIG.RefVec.empty |>.push ref
+    ⟨⟨aig, ⟩, sorry⟩
+  | .zeroExtend (w := w) v inner =>
+    let ⟨⟨aig, evec⟩, haig⟩ := BVExpr.bitblast.go aig inner
+    let res := BVExpr.bitblast.blastZeroExtend aig ⟨w, evec⟩
+    have := by
+      apply AIG.LawfulVecOperator.le_size_of_le_aig_size (f := BVExpr.bitblast.blastZeroExtend)
+      dsimp only at haig
+      assumption
+    ⟨res, this⟩
+  | .signExtend (w := w) v inner =>
+    let ⟨⟨aig, evec⟩, haig⟩ := BVExpr.bitblast.go aig inner
+    let res := BVExpr.bitblast.blastSignExtend aig ⟨w, evec⟩
+    have := by
+      apply AIG.LawfulVecOperator.le_size_of_le_aig_size (f := BVExpr.bitblast.blastSignExtend)
+      dsimp only at haig
+      assumption
+    ⟨res, this⟩
+  | .bin lhs op rhs =>
+    let ⟨⟨aig, lhs⟩, hlaig⟩ := BVExpr.bitblast.go aig lhs
+    let ⟨⟨aig, rhs⟩, hraig⟩ := BVExpr.bitblast.go aig rhs
+    let lhs := lhs.cast <| by
+      dsimp only at hlaig hraig
+      omega
+    match op with
+    | .and =>
+       let res := AIG.RefVec.zip aig ⟨⟨lhs, rhs⟩, AIG.mkAndCached⟩
+       have := by
+         apply AIG.LawfulVecOperator.le_size_of_le_aig_size (f := AIG.RefVec.zip)
+         dsimp only at hlaig hraig
+         omega
+       ⟨res, this⟩
+    | .or =>
+       let res := AIG.RefVec.zip aig ⟨⟨lhs, rhs⟩, AIG.mkOrCached⟩
+       have := by
+         apply AIG.LawfulVecOperator.le_size_of_le_aig_size (f := AIG.RefVec.zip)
+         dsimp only at hlaig hraig
+         omega
+       ⟨res, this⟩
+    | .xor =>
+       let res := AIG.RefVec.zip aig ⟨⟨lhs, rhs⟩, AIG.mkXorCached⟩
+       have := by
+         apply AIG.LawfulVecOperator.le_size_of_le_aig_size (f := AIG.RefVec.zip)
+         dsimp only at hlaig hraig
+         omega
+       ⟨res, this⟩
+    | .add =>
+      let res := BVExpr.bitblast.blastAdd aig ⟨lhs, rhs⟩
+      have := by
+        apply AIG.LawfulVecOperator.le_size_of_le_aig_size (f := BVExpr.bitblast.blastAdd)
+        dsimp only at hlaig hraig
+        omega
+      ⟨res, this⟩
+    | .mul =>
+      let res := BVExpr.bitblast.blastMul aig ⟨lhs, rhs⟩
+      have := by
+        apply AIG.LawfulVecOperator.le_size_of_le_aig_size (f := BVExpr.bitblast.blastMul)
+        dsimp only at hlaig hraig
+        omega
+      ⟨res, this⟩
+    | .udiv =>
+      let res := BVExpr.bitblast.blastUdiv aig ⟨lhs, rhs⟩
+      have := by
+        apply AIG.LawfulVecOperator.le_size_of_le_aig_size (f := BVExpr.bitblast.blastUdiv)
+        dsimp only at hlaig hraig
+        omega
+      ⟨res, this⟩
+    | .umod =>
+      let res := BVExpr.bitblast.blastUmod aig ⟨lhs, rhs⟩
+      have := by
+        apply AIG.LawfulVecOperator.le_size_of_le_aig_size (f := BVExpr.bitblast.blastUmod)
+        dsimp only at hlaig hraig
+        omega
+      ⟨res, this⟩
+  | .un op expr =>
+    let ⟨⟨eaig, evec⟩, heaig⟩ := BVExpr.bitblast.go aig expr
+    match op with
+    | .not =>
+        let res := BVExpr.bitblast.blastNot eaig evec
+        have := by
+          apply AIG.LawfulVecOperator.le_size_of_le_aig_size (f := AIG.RefVec.map)
+          dsimp only at heaig
+          omega
+        ⟨res, this⟩
+    | .shiftLeftConst distance =>
+      let res := BVExpr.bitblast.blastShiftLeftConst eaig ⟨evec, distance⟩
+      have := by
+        apply AIG.LawfulVecOperator.le_size_of_le_aig_size (f := BVExpr.bitblast.blastShiftLeftConst)
+        dsimp only at heaig
+        assumption
+      ⟨res, this⟩
+    | .shiftRightConst distance =>
+      let res := BVExpr.bitblast.blastShiftRightConst eaig ⟨evec, distance⟩
+      have := by
+        apply AIG.LawfulVecOperator.le_size_of_le_aig_size (f := BVExpr.bitblast.blastShiftRightConst)
+        dsimp only at heaig
+        assumption
+      ⟨res, this⟩
+    | .rotateLeft distance =>
+      let res := BVExpr.bitblast.blastRotateLeft eaig ⟨evec, distance⟩
+      have := by
+        apply AIG.LawfulVecOperator.le_size_of_le_aig_size (f := BVExpr.bitblast.blastRotateLeft)
+        dsimp only at heaig
+        assumption
+      ⟨res, this⟩
+    | .rotateRight distance =>
+      let res := BVExpr.bitblast.blastRotateRight eaig ⟨evec, distance⟩
+      have := by
+        apply AIG.LawfulVecOperator.le_size_of_le_aig_size (f := BVExpr.bitblast.blastRotateRight)
+        dsimp only at heaig
+        assumption
+      ⟨res, this⟩
+    | .arithShiftRightConst distance =>
+      let res := BVExpr.bitblast.blastArithShiftRightConst eaig ⟨evec, distance⟩
+      have := by
+        apply AIG.LawfulVecOperator.le_size_of_le_aig_size (f := BVExpr.bitblast.blastArithShiftRightConst)
+        dsimp only at heaig
+        assumption
+      ⟨res, this⟩
+  | .append lhs rhs =>
+    let ⟨⟨aig, lhs⟩, hlaig⟩ := BVExpr.bitblast.go aig lhs
+    let ⟨⟨aig, rhs⟩, hraig⟩ := BVExpr.bitblast.go aig rhs
+    let lhs := lhs.cast <| by
+      dsimp only at hlaig hraig
+      omega
+    let res := BVExpr.bitblast.blastAppend aig ⟨lhs, rhs, by ac_rfl⟩
+    have := by
+      apply AIG.LawfulVecOperator.le_size_of_le_aig_size (f := BVExpr.bitblast.blastAppend)
+      dsimp only at hlaig hraig
+      omega
+    ⟨res, this⟩
+  | .replicate n expr =>
+    let ⟨⟨aig, expr⟩, haig⟩ := BVExpr.bitblast.go aig expr
+    let res := BVExpr.bitblast.blastReplicate aig ⟨n, expr, rfl⟩
+    have := by
+      apply AIG.LawfulVecOperator.le_size_of_le_aig_size (f := BVExpr.bitblast.blastReplicate)
+      dsimp only at haig
+      assumption
+    ⟨res, this⟩
+  | .extract start len expr =>
+    let ⟨⟨eaig, evec⟩, heaig⟩ := BVExpr.bitblast.go aig expr
+    let res := BVExpr.bitblast.blastExtract eaig ⟨evec, start⟩
+    have := by
+      apply AIG.LawfulVecOperator.le_size_of_le_aig_size (f := BVExpr.bitblast.blastExtract)
+      dsimp only at heaig
+      exact heaig
+    ⟨res, this⟩
+  | .shiftLeft lhs rhs =>
+    let ⟨⟨aig, lhs⟩, hlaig⟩ := BVExpr.bitblast.go aig lhs
+    let ⟨⟨aig, rhs⟩, hraig⟩ := BVExpr.bitblast.go aig rhs
+    let lhs := lhs.cast <| by
+      dsimp only at hlaig hraig
+      omega
+    let res := BVExpr.bitblast.blastShiftLeft aig ⟨_, lhs, rhs⟩
+    have := by
+      apply AIG.LawfulVecOperator.le_size_of_le_aig_size (f := BVExpr.bitblast.blastShiftLeft)
+      dsimp only at hlaig hraig
+      omega
+    ⟨res, this⟩
+  | .shiftRight lhs rhs =>
+    let ⟨⟨aig, lhs⟩, hlaig⟩ := BVExpr.bitblast.go aig lhs
+    let ⟨⟨aig, rhs⟩, hraig⟩ := BVExpr.bitblast.go aig rhs
+    let lhs := lhs.cast <| by
+      dsimp only at hlaig hraig
+      omega
+    let res := BVExpr.bitblast.blastShiftRight aig ⟨_, lhs, rhs⟩
+    have := by
+      apply AIG.LawfulVecOperator.le_size_of_le_aig_size (f := BVExpr.bitblast.blastShiftRight)
+      dsimp only at hlaig hraig
+      omega
+    ⟨res, this⟩
+
+def BVPred.bitblast.go (aig : AIG BVBit) (pred : BVPred) : AIG.ExtendingEntrypoint aig :=
+  match pred with
+  | .bin lhs op rhs =>
+    let ⟨res, _⟩ := BVExpr.bitblast.go aig lhs
+    let aig := res.aig
+    let lhsRefs := res.vec
+    let ⟨res, _⟩ := BVExpr.bitblast.go aig rhs
+    let aig := res.aig
+    let rhsRefs := res.vec
+    let lhsRefs := lhsRefs.cast <| sorry
+    match op with
+    | .eq => ⟨BVPred.mkEq aig ⟨lhsRefs, rhsRefs⟩, sorry⟩
+    | .ult => ⟨BVPred.mkUlt aig ⟨lhsRefs, rhsRefs⟩, sorry⟩
+  | .getLsbD expr idx =>
+    /-
+    Note: This blasts the entire expression up to `w` despite only needing it up to `idx`.
+    However the vast majority of operations are interested in all bits so the API is currently
+    not designed to support this use case.
+    -/
+    let ⟨res, _⟩ := BVExpr.bitblast.go aig expr
+    let aig := res.aig
+    let refs := res.vec
+    ⟨BVPred.blastGetLsbD aig ⟨refs, idx⟩, sorry⟩
+
+def BVLogicalExpr.bitblast.go (aig : AIG BVBit) (expr : BVLogicalExpr) : AIG.ExtendingEntrypoint aig :=
+  match expr with
+  | .literal pred => BVPred.bitblast.go aig pred
+  | .const val => ⟨aig.mkConstCached val, (by apply AIG.LawfulOperator.le_size)⟩
+  | .not expr =>
+    let ⟨⟨aig, exprRef⟩, _⟩ := BVLogicalExpr.bitblast.go aig expr
+    let ret := aig.mkNotCached exprRef
+    have := AIG.LawfulOperator.le_size (f := AIG.mkNotCached) aig exprRef
+    ⟨ret, by dsimp only [ret] at *; omega⟩
+  | .gate g lhs rhs =>
+    let ⟨⟨aig, lhsRef⟩, lextend⟩ := BVLogicalExpr.bitblast.go aig lhs
+    let ⟨⟨aig, rhsRef⟩, rextend⟩ := BVLogicalExpr.bitblast.go aig rhs
+    let lhsRef := lhsRef.cast <| by
+      dsimp only at rextend ⊢
+      omega
+    let input := ⟨lhsRef, rhsRef⟩
+    match g with
+    | .and =>
+      let ret := aig.mkAndCached input
+      have := AIG.LawfulOperator.le_size (f := AIG.mkAndCached) aig input
+      ⟨ret, by dsimp only [ret] at lextend rextend ⊢; omega⟩
+    | .xor =>
+      let ret := aig.mkXorCached input
+      have := AIG.LawfulOperator.le_size (f := AIG.mkXorCached) aig input
+      ⟨ret, by dsimp only [ret] at lextend rextend ⊢; omega⟩
+    | .beq =>
+      let ret := aig.mkBEqCached input
+      have := AIG.LawfulOperator.le_size (f := AIG.mkBEqCached) aig input
+      ⟨ret, by dsimp only [ret] at lextend rextend ⊢; omega⟩
+
+end
+
+
+namespace BVExpr
+
+def bitblast (aig : AIG BVBit) (expr : BVExpr w) : AIG.RefVecEntry BVBit w :=
+  bitblast.go aig expr |>.val
+
+theorem bitblast.go_decl_eq (aig : AIG BVBit) (expr : BVExpr w) :
+    ∀ (idx : Nat) (h1) (h2), (go aig expr).val.aig.decls[idx]'h2 = aig.decls[idx]'h1 := by
+  intros idx h1 h2
+  sorry
+/-
+  induction expr generalizing aig with
+  | var =>
+    dsimp only [go]
+    rw [AIG.LawfulVecOperator.decl_eq (f := blastVar)]
+  | const =>
+    dsimp only [go]
+    rw [AIG.LawfulVecOperator.decl_eq (f := blastConst)]
+  | ofBool => sorry
+  | bin lhs op rhs lih rih =>
+    match op with
+    | .and | .or | .xor | .add | .mul | .udiv | .umod =>
+      dsimp only [go]
+      have := (bitblast.go aig lhs).property
+      have := (go (go aig lhs).1.aig rhs).property
+      have := (bitblast.go aig lhs).property
+      rw [AIG.LawfulVecOperator.decl_eq]
+      rw [rih, lih]
+      · omega
+      · apply Nat.lt_of_lt_of_le h1 -- omega cannot do this :(
+        apply Nat.le_trans <;> assumption
+  | un op expr ih =>
+    match op with
+    | .not | .shiftLeftConst .. | .shiftRightConst .. | .rotateLeft .. | .rotateRight ..
+    | .arithShiftRightConst .. =>
+      dsimp only [go]
+      rw [AIG.LawfulVecOperator.decl_eq]
+      rw [ih]
+      have := (go aig expr).property
+      omega
+  | zeroExtend w inner ih =>
+    dsimp only [go]
+    rw [AIG.LawfulVecOperator.decl_eq (f := blastZeroExtend)]
+    rw [ih]
+    have := (go aig inner).property
+    omega
+  | signExtend w inner ih =>
+    dsimp only [go]
+    rw [AIG.LawfulVecOperator.decl_eq (f := blastSignExtend)]
+    rw [ih]
+    have := (go aig inner).property
+    omega
+  | append lhs rhs lih rih =>
+    dsimp only [go]
+    have := (bitblast.go aig lhs).property
+    have := (bitblast.go aig lhs).property
+    have := (go (go aig lhs).1.aig rhs).property
+    rw [AIG.LawfulVecOperator.decl_eq (f := blastAppend)]
+    rw [rih, lih]
+    · omega
+    · apply Nat.lt_of_lt_of_le h1
+      apply Nat.le_trans <;> assumption
+  | replicate n inner ih =>
+    dsimp only [go]
+    rw [AIG.LawfulVecOperator.decl_eq (f := blastReplicate)]
+    rw [ih]
+    have := (go aig inner).property
+    omega
+  | extract hi lo inner ih =>
+    dsimp only [go]
+    rw [AIG.LawfulVecOperator.decl_eq (f := blastExtract)]
+    rw [ih]
+    have := (go aig inner).property
+    omega
+  | shiftLeft lhs rhs lih rih =>
+    dsimp only [go]
+    have := (bitblast.go aig lhs).property
+    have := (bitblast.go aig lhs).property
+    have := (go (go aig lhs).1.aig rhs).property
+    rw [AIG.LawfulVecOperator.decl_eq (f := blastShiftLeft)]
+    rw [rih, lih]
+    · omega
+    · apply Nat.lt_of_lt_of_le h1
+      apply Nat.le_trans <;> assumption
+  | shiftRight lhs rhs lih rih =>
+    dsimp only [go]
+    have := (bitblast.go aig lhs).property
+    have := (bitblast.go aig lhs).property
+    have := (go (go aig lhs).1.aig rhs).property
+    rw [AIG.LawfulVecOperator.decl_eq (f := blastShiftRight)]
+    rw [rih, lih]
+    · omega
+    · apply Nat.lt_of_lt_of_le h1
+      apply Nat.le_trans <;> assumption
+  -/
+
+instance : AIG.LawfulVecOperator BVBit (fun _ w => BVExpr w) bitblast where
+  le_size := by
+    intro _ aig expr
+    unfold bitblast
+    exact (bitblast.go aig expr).property
+  decl_eq := by
+    intros
+    unfold bitblast
+    apply bitblast.go_decl_eq
+
+end BVExpr
+
+namespace BVPred
+
+def bitblast (aig : AIG BVBit) (pred : BVPred) : AIG.Entrypoint BVBit :=
+  bitblast.go aig pred |>.val
+
+instance : AIG.LawfulOperator BVBit (fun _ => BVPred) bitblast where
+  le_size := by sorry
+    /-
+    intro aig pred
+    unfold bitblast
+    cases pred with
+    | bin lhs op rhs =>
+      cases op with
+      | eq =>
+        apply AIG.LawfulOperator.le_size_of_le_aig_size (f := mkEq)
+        apply AIG.LawfulVecOperator.le_size_of_le_aig_size (f := BVExpr.bitblast)
+        apply AIG.LawfulVecOperator.le_size (f := BVExpr.bitblast)
+      | ult =>
+        apply AIG.LawfulOperator.le_size_of_le_aig_size (f := mkUlt)
+        apply AIG.LawfulVecOperator.le_size_of_le_aig_size (f := BVExpr.bitblast)
+        apply AIG.LawfulVecOperator.le_size (f := BVExpr.bitblast)
+    | getLsbD expr idx =>
+      apply AIG.LawfulOperator.le_size_of_le_aig_size (f := blastGetLsbD)
+      apply AIG.LawfulVecOperator.le_size (f := BVExpr.bitblast)
+    -/
+  decl_eq := by sorry
+    /-
+    intro aig pred idx h1 h2
+    cases pred with
+    | bin lhs op rhs =>
+      cases op with
+      | eq =>
+        simp only [bitblast]
+        rw [AIG.LawfulOperator.decl_eq (f := mkEq)]
+        rw [AIG.LawfulVecOperator.decl_eq (f := BVExpr.bitblast)]
+        rw [AIG.LawfulVecOperator.decl_eq (f := BVExpr.bitblast)]
+        · apply AIG.LawfulVecOperator.lt_size_of_lt_aig_size (f := BVExpr.bitblast)
+          assumption
+        · apply AIG.LawfulVecOperator.lt_size_of_lt_aig_size (f := BVExpr.bitblast)
+          apply AIG.LawfulVecOperator.le_size_of_le_aig_size (f := BVExpr.bitblast)
+          assumption
+      | ult =>
+        simp only [bitblast]
+        rw [AIG.LawfulOperator.decl_eq (f := mkUlt)]
+        rw [AIG.LawfulVecOperator.decl_eq (f := BVExpr.bitblast)]
+        rw [AIG.LawfulVecOperator.decl_eq (f := BVExpr.bitblast)]
+        · apply AIG.LawfulVecOperator.lt_size_of_lt_aig_size (f := BVExpr.bitblast)
+          assumption
+        · apply AIG.LawfulVecOperator.lt_size_of_lt_aig_size (f := BVExpr.bitblast)
+          apply AIG.LawfulVecOperator.le_size_of_le_aig_size (f := BVExpr.bitblast)
+          assumption
+    | getLsbD expr idx =>
+      simp only [bitblast]
+      rw [AIG.LawfulOperator.decl_eq (f := blastGetLsbD)]
+      rw [AIG.LawfulVecOperator.decl_eq (f := BVExpr.bitblast)]
+      apply AIG.LawfulVecOperator.lt_size_of_lt_aig_size (f := BVExpr.bitblast)
+      assumption
+    -/
+
+end BVPred
+
 
 namespace BVLogicalExpr
 
-def bitblast (expr : BVLogicalExpr) : Entrypoint BVBit :=
-  go AIG.empty expr |>.val
-where
-  go (aig : AIG BVBit) (expr : BVLogicalExpr) : ExtendingEntrypoint aig :=
-    match expr with
-    | .literal pred => ⟨BVPred.bitblast aig pred, by apply LawfulOperator.le_size⟩
-    | .const val => ⟨aig.mkConstCached val, (by apply LawfulOperator.le_size)⟩
-    | .not expr =>
-      let ⟨⟨aig, exprRef⟩, _⟩ := go aig expr
-      let ret := aig.mkNotCached exprRef
-      have := LawfulOperator.le_size (f := mkNotCached) aig exprRef
-      ⟨ret, by dsimp only [ret] at *; omega⟩
-    | .gate g lhs rhs =>
-      let ⟨⟨aig, lhsRef⟩, lextend⟩ := go aig lhs
-      let ⟨⟨aig, rhsRef⟩, rextend⟩ := go aig rhs
-      let lhsRef := lhsRef.cast <| by
-        dsimp only at rextend ⊢
-        omega
-      let input := ⟨lhsRef, rhsRef⟩
-      match g with
-      | .and =>
-        let ret := aig.mkAndCached input
-        have := LawfulOperator.le_size (f := mkAndCached) aig input
-        ⟨ret, by dsimp only [ret] at lextend rextend ⊢; omega⟩
-      | .xor =>
-        let ret := aig.mkXorCached input
-        have := LawfulOperator.le_size (f := mkXorCached) aig input
-        ⟨ret, by dsimp only [ret] at lextend rextend ⊢; omega⟩
-      | .beq =>
-        let ret := aig.mkBEqCached input
-        have := LawfulOperator.le_size (f := mkBEqCached) aig input
-        ⟨ret, by dsimp only [ret] at lextend rextend ⊢; omega⟩
+def bitblast (expr : BVLogicalExpr) : AIG.Entrypoint BVBit :=
+  bitblast.go AIG.empty expr |>.val
 
 namespace bitblast
 
@@ -66,6 +474,8 @@ theorem go_decls_size_le (expr : BVLogicalExpr) (aig : AIG BVBit) :
 
 theorem go_decl_eq (idx) (aig : AIG BVBit) (h : idx < aig.decls.size) (hbounds) :
     (bitblast.go aig expr).val.aig.decls[idx]'hbounds = aig.decls[idx] := by
+  sorry
+  /-
   induction expr generalizing aig with
   | const =>
     simp only [go]
@@ -94,14 +504,15 @@ theorem go_decl_eq (idx) (aig : AIG BVBit) (h : idx < aig.decls.size) (hbounds) 
     | beq =>
       simp only [go]
       rw [AIG.LawfulOperator.decl_eq (f := mkBEqCached), rih, lih]
+    -/
 
-theorem go_isPrefix_aig {aig : AIG BVBit} :
-    IsPrefix aig.decls (go aig expr).val.aig.decls := by
-  apply IsPrefix.of
+theorem go_isPrefix_aig {aig : AIG BVBit} : AIG.IsPrefix aig.decls (go aig expr).val.aig.decls := by
+  apply AIG.IsPrefix.of
   · intro idx h
     apply go_decl_eq
   · apply go_decls_size_le
 
+open AIG in
 @[simp]
 theorem go_denote_entry (entry : Entrypoint BVBit) {h} :
     ⟦(go entry.aig expr).val.aig, ⟨entry.ref.gate, h⟩, assign⟧ = ⟦entry, assign⟧ := by
